Add method for initializing disk with a nonzero size
Also add framework to initialize disks in semantic tests, and add new
semantics tests. The generated_tests file takes a long time now: we
should probably split the WAL tests from the rest of the semantics
tests, or find another way to improve performance

src/goose_lang/examples/goose_semantics.v
@@ -94,14 +94,23 @@ Definition testCopySimple: val :=
     SliceCopy byteT "y" "x";;
     (SliceGet byteT "y" #3 = #(U8 1)).
 
-Definition testCopyDifferentLengths: val :=
-  rec: "testCopyDifferentLengths" <> :=
+Definition testCopyShorterDst: val :=
+  rec: "testCopyShorterDst" <> :=
     let: "x" := NewSlice byteT #15 in
     SliceSet byteT "x" #3 (#(U8 1));;
     SliceSet byteT "x" #12 (#(U8 2));;
     let: "y" := NewSlice byteT #10 in
     let: "n" := SliceCopy byteT "y" "x" in
     ("n" = #10) && (SliceGet byteT "y" #3 = #(U8 1)).
+
+Definition testCopyShorterSrc: val :=
+  rec: "testCopyShorterSrc" <> :=
+    let: "x" := NewSlice byteT #10 in
+    let: "y" := NewSlice byteT #15 in
+    SliceSet byteT "x" #3 (#(U8 1));;
+    SliceSet byteT "y" #12 (#(U8 2));;
+    let: "n" := SliceCopy byteT "y" "x" in
+    ("n" = #10) && (SliceGet byteT "y" #3 = #(U8 1)) && (SliceGet byteT "y" #12 = #(U8 2)).
 
 (* encoding.go *)
 
@@ -270,6 +279,17 @@ Definition failing_testFunctionOrdering: val :=
                 then #false
                 else (struct.get Pair.S "x" "p" + struct.get Pair.S "x" "q" = #109)))))))).
 
+(* lock.go *)
+
+(* We can't interpret multithreaded code, so this just checks that
+   locks are correctly interpreted *)
+Definition testsUseLocks: val :=
+  rec: "testsUseLocks" <> :=
+    let: "m" := lock.new #() in
+    lock.acquire "m";;
+    lock.release "m";;
+    #true.
+
 (* loops.go *)
 
 (* helpers *)
@@ -350,6 +370,39 @@ Definition failing_testBreakFromLoopNoContinue: val :=
       Continue);;
     (![uint64T] "i" = #1).
 
+Definition testNestedLoops: val :=
+  rec: "testNestedLoops" <> :=
+    let: "ok1" := ref_to boolT #false in
+    let: "ok2" := ref_to boolT #false in
+    let: "i" := ref_to uint64T #0 in
+    (for: (λ: <>, #true); (λ: <>, Skip) := λ: <>,
+      let: "j" := ref_to uint64T #0 in
+      (for: (λ: <>, #true); (λ: <>, Skip) := λ: <>,
+        (if: ![uint64T] "j" > #5
+        then Break
+        else
+          "j" <-[uint64T] ![uint64T] "j" + #1;;
+          "ok1" <-[boolT] (![uint64T] "j" = #6);;
+          Continue));;
+      "i" <-[uint64T] ![uint64T] "i" + #1;;
+      "ok2" <-[boolT] (![uint64T] "i" = #1);;
+      Break);;
+    ![boolT] "ok1" && ![boolT] "ok2".
+
+Definition testNestedGoStyleLoops: val :=
+  rec: "testNestedGoStyleLoops" <> :=
+    let: "ok" := ref_to boolT #false in
+    let: "i" := ref_to uint64T #0 in
+    (for: (λ: <>, ![uint64T] "i" < #10); (λ: <>, "i" <-[uint64T] ![uint64T] "i" + #1) := λ: <>,
+      let: "j" := ref_to uint64T #0 in
+      (for: (λ: <>, ![uint64T] "j" < ![uint64T] "i"); (λ: <>, "j" <-[uint64T] ![uint64T] "j" + #1) := λ: <>,
+        (if: #true
+        then Break
+        else Continue));;
+      "ok" <-[boolT] (![uint64T] "i" = #9);;
+      Continue);;
+    ![boolT] "ok".
+
 (* maps.go *)
 
 Definition IterateMapKeys: val :=
@@ -387,6 +440,18 @@ Definition testMapSize: val :=
     MapInsert "m" #3 #4;;
     "ok" <-[boolT] ![boolT] "ok" && (MapLen "m" = #3);;
     ![boolT] "ok".
+
+(* nil.go *)
+
+Definition failing_testCompareSliceToNil: val :=
+  rec: "failing_testCompareSliceToNil" <> :=
+    let: "s" := NewSlice byteT #0 in
+    "s" ≠ slice.nil.
+
+Definition testComparePointerToNil: val :=
+  rec: "testComparePointerToNil" <> :=
+    let: "s" := ref (zero_val uint64T) in
+    "s" ≠ slice.nil.
 
 (* operations.go *)
 
@@ -784,3 +849,199 @@ Definition testStoreInStructPointerVar: val :=
     let: "p" := ref_to (refT (struct.t StructWrap.S)) (struct.alloc StructWrap.S (zero_val (struct.t StructWrap.S))) in
     struct.storeF StructWrap.S "i" (![refT (struct.t StructWrap.S)] "p") #5;;
     (struct.loadF StructWrap.S "i" (![refT (struct.t StructWrap.S)] "p") = #5).
+
+(* wal.go *)
+
+(* 10 is completely arbitrary *)
+Definition MaxTxnWrites : expr := #10.
+
+Definition logLength : expr := #1 + #2 * MaxTxnWrites.
+
+Module Log.
+  Definition S := struct.decl [
+    "d" :: disk.Disk;
+    "l" :: lockRefT;
+    "cache" :: mapT disk.blockT;
+    "length" :: refT uint64T
+  ].
+End Log.
+
+Definition intToBlock: val :=
+  rec: "intToBlock" "a" :=
+    let: "b" := NewSlice byteT disk.BlockSize in
+    UInt64Put "b" "a";;
+    "b".
+
+Definition blockToInt: val :=
+  rec: "blockToInt" "v" :=
+    let: "a" := UInt64Get "v" in
+    "a".
+
+(* New initializes a fresh log *)
+Definition New: val :=
+  rec: "New" <> :=
+    let: "d" := disk.Get #() in
+    let: "diskSize" := disk.Size #() in
+    (if: "diskSize" ≤ logLength
+    then
+      Panic ("disk is too small to host log");;
+      #()
+    else #());;
+    let: "cache" := NewMap disk.blockT in
+    let: "header" := intToBlock #0 in
+    disk.Write #0 "header";;
+    let: "lengthPtr" := ref (zero_val uint64T) in
+    "lengthPtr" <-[refT uint64T] #0;;
+    let: "l" := lock.new #() in
+    struct.mk Log.S [
+      "d" ::= "d";
+      "cache" ::= "cache";
+      "length" ::= "lengthPtr";
+      "l" ::= "l"
+    ].
+
+Definition Log__lock: val :=
+  rec: "Log__lock" "l" :=
+    lock.acquire (struct.get Log.S "l" "l").
+
+Definition Log__unlock: val :=
+  rec: "Log__unlock" "l" :=
+    lock.release (struct.get Log.S "l" "l").
+
+(* BeginTxn allocates space for a new transaction in the log.
+
+   Returns true if the allocation succeeded. *)
+Definition Log__BeginTxn: val :=
+  rec: "Log__BeginTxn" "l" :=
+    Log__lock "l";;
+    let: "length" := ![uint64T] (struct.get Log.S "length" "l") in
+    (if: ("length" = #0)
+    then
+      Log__unlock "l";;
+      #true
+    else
+      Log__unlock "l";;
+      #false).
+
+(* Read from the logical disk.
+
+   Reads must go through the log to return committed but un-applied writes. *)
+Definition Log__Read: val :=
+  rec: "Log__Read" "l" "a" :=
+    Log__lock "l";;
+    let: ("v", "ok") := MapGet (struct.get Log.S "cache" "l") "a" in
+    (if: "ok"
+    then
+      Log__unlock "l";;
+      "v"
+    else
+      Log__unlock "l";;
+      let: "dv" := disk.Read (logLength + "a") in
+      "dv").
+
+Definition Log__Size: val :=
+  rec: "Log__Size" "l" :=
+    let: "sz" := disk.Size #() in
+    "sz" - logLength.
+
+(* Write to the disk through the log. *)
+Definition Log__Write: val :=
+  rec: "Log__Write" "l" "a" "v" :=
+    Log__lock "l";;
+    let: "length" := ![uint64T] (struct.get Log.S "length" "l") in
+    (if: "length" ≥ MaxTxnWrites
+    then
+      Panic ("transaction is at capacity");;
+      #()
+    else #());;
+    let: "aBlock" := intToBlock "a" in
+    let: "nextAddr" := #1 + #2 * "length" in
+    disk.Write "nextAddr" "aBlock";;
+    disk.Write ("nextAddr" + #1) "v";;
+    MapInsert (struct.get Log.S "cache" "l") "a" "v";;
+    struct.get Log.S "length" "l" <-[refT uint64T] "length" + #1;;
+    Log__unlock "l".
+
+(* Commit the current transaction. *)
+Definition Log__Commit: val :=
+  rec: "Log__Commit" "l" :=
+    Log__lock "l";;
+    let: "length" := ![uint64T] (struct.get Log.S "length" "l") in
+    Log__unlock "l";;
+    let: "header" := intToBlock "length" in
+    disk.Write #0 "header".
+
+Definition getLogEntry: val :=
+  rec: "getLogEntry" "d" "logOffset" :=
+    let: "diskAddr" := #1 + #2 * "logOffset" in
+    let: "aBlock" := disk.Read "diskAddr" in
+    let: "a" := blockToInt "aBlock" in
+    let: "v" := disk.Read ("diskAddr" + #1) in
+    ("a", "v").
+
+(* applyLog assumes we are running sequentially *)
+Definition applyLog: val :=
+  rec: "applyLog" "d" "length" :=
+    let: "i" := ref_to uint64T #0 in
+    (for: (λ: <>, #true); (λ: <>, Skip) := λ: <>,
+      (if: ![uint64T] "i" < "length"
+      then
+        let: ("a", "v") := getLogEntry "d" (![uint64T] "i") in
+        disk.Write (logLength + "a") "v";;
+        "i" <-[uint64T] ![uint64T] "i" + #1;;
+        Continue
+      else Break)).
+
+Definition clearLog: val :=
+  rec: "clearLog" "d" :=
+    let: "header" := intToBlock #0 in
+    disk.Write #0 "header".
+
+(* Apply all the committed transactions.
+
+   Frees all the space in the log. *)
+Definition Log__Apply: val :=
+  rec: "Log__Apply" "l" :=
+    Log__lock "l";;
+    let: "length" := ![uint64T] (struct.get Log.S "length" "l") in
+    applyLog (struct.get Log.S "d" "l") "length";;
+    clearLog (struct.get Log.S "d" "l");;
+    struct.get Log.S "length" "l" <-[refT uint64T] #0;;
+    Log__unlock "l".
+
+(* Open recovers the log following a crash or shutdown *)
+Definition Open: val :=
+  rec: "Open" <> :=
+    let: "d" := disk.Get #() in
+    let: "header" := disk.Read #0 in
+    let: "length" := blockToInt "header" in
+    applyLog "d" "length";;
+    clearLog "d";;
+    let: "cache" := NewMap disk.blockT in
+    let: "lengthPtr" := ref (zero_val uint64T) in
+    "lengthPtr" <-[refT uint64T] #0;;
+    let: "l" := lock.new #() in
+    struct.mk Log.S [
+      "d" ::= "d";
+      "cache" ::= "cache";
+      "length" ::= "lengthPtr";
+      "l" ::= "l"
+    ].
+
+(* test *)
+Definition testWal: val :=
+  rec: "testWal" <> :=
+    let: "ok" := ref_to boolT #true in
+    let: "lg" := New #() in
+    (if: Log__BeginTxn "lg"
+    then
+      Log__Write "lg" #2 (intToBlock #11);;
+      #()
+    else #());;
+    "ok" <-[boolT] ![boolT] "ok" && (blockToInt (Log__Read "lg" #2) = #11);;
+    "ok" <-[boolT] ![boolT] "ok" && (blockToInt (disk.Read #0) = #0);;
+    Log__Commit "lg";;
+    "ok" <-[boolT] ![boolT] "ok" && (blockToInt (disk.Read #0) = #1);;
+    Log__Apply "lg";;
+    "ok" <-[boolT] ![boolT] "ok" && (![uint64T] (struct.get Log.S "length" "lg") = #0);;
+    ![boolT] "ok".
